wip

code/k256/Hacl.Impl.K256.GLV.fst
@@ -28,64 +28,73 @@ open Hacl.Impl.K256.GLV.Constants
 
 #set-options "--z3rlimit 50 --fuel 0 --ifuel 0"
 
+(**
+  Representing a scalar k as (r1 + r2 * lambda) mod S.q,
+  s.t. r1 and r2 are ~128 bits long
+*)
+
 inline_for_extraction noextract
-val scalar_split_lambda_g1g2 (tmp1 tmp2 k1 k2 k: qelem) : Stack unit
+val scalar_split_lambda_g1g2 (tmp1 tmp2 r1 r2 k: qelem) : Stack unit
   (requires fun h ->
-    live h k /\ live h k1 /\ live h k2 /\
+    live h k /\ live h r1 /\ live h r2 /\
     live h tmp1 /\ live h tmp2 /\
-    disjoint k k1 /\ disjoint k k2 /\ disjoint k1 k2 /\
-    disjoint tmp1 k1 /\ disjoint tmp1 k2 /\ disjoint tmp1 k /\
-    disjoint tmp2 k1 /\ disjoint tmp2 k2 /\ disjoint tmp2 k /\
+    disjoint k r1 /\ disjoint k r2 /\ disjoint r1 r2 /\
+    disjoint tmp1 r1 /\ disjoint tmp1 r2 /\ disjoint tmp1 k /\
+    disjoint tmp2 r1 /\ disjoint tmp2 r2 /\ disjoint tmp2 k /\
     disjoint tmp1 tmp2 /\ qas_nat h k < S.q)
   (ensures  fun h0 _ h1 ->
-    modifies (loc k1 |+| loc k2 |+| loc tmp1 |+| loc tmp2) h0 h1 /\
-   (let k1 = qas_nat h1 k1 in let k2 = qas_nat h1 k2 in
-    k1 < S.q /\ k1 = SG.qmul_shift_384 (qas_nat h0 k) SG.g1 /\
-    k2 < S.q /\ k2 = SG.qmul_shift_384 (qas_nat h0 k) SG.g2))
+    modifies (loc r1 |+| loc r2 |+| loc tmp1 |+| loc tmp2) h0 h1 /\
+   (let r1 = qas_nat h1 r1 in let r2 = qas_nat h1 r2 in
+    r1 < S.q /\ r1 = SG.qmul_shift_384 (qas_nat h0 k) SG.g1 /\
+    r2 < S.q /\ r2 = SG.qmul_shift_384 (qas_nat h0 k) SG.g2))
 
-let scalar_split_lambda_g1g2 tmp1 tmp2 k1 k2 k =
+let scalar_split_lambda_g1g2 tmp1 tmp2 r1 r2 k =
   make_g1 tmp1; // tmp1 = g1
   make_g2 tmp2; // tmp2 = g2
-  qmul_shift_384 k1 k tmp1; // k1 = c1 = qmul_shift_384 k g1
-  qmul_shift_384 k2 k tmp2; // k2 = c2 = qmul_shift_384 k g2
+  qmul_shift_384 r1 k tmp1; // r1 = c1 = qmul_shift_384 k g1
+  qmul_shift_384 r2 k tmp2; // r2 = c2 = qmul_shift_384 k g2
   let h0 = ST.get () in
   SG.qmul_shift_384_lemma (qas_nat h0 k) (qas_nat h0 tmp1);
   SG.qmul_shift_384_lemma (qas_nat h0 k) (qas_nat h0 tmp2);
-  assert (qas_nat h0 k1 < S.q /\ qas_nat h0 k2 < S.q)
+  assert (qas_nat h0 r1 < S.q /\ qas_nat h0 r2 < S.q)
 
 
-// k = (k1 + lambda * k2) % S.q
-val scalar_split_lambda (k1 k2 k: qelem) : Stack unit
+// k = (r1 + lambda * k2) % S.q
+val scalar_split_lambda (r1 r2 k: qelem) : Stack unit
   (requires fun h ->
-    live h k /\ live h k1 /\ live h k2 /\
-    disjoint k k1 /\ disjoint k k2 /\ disjoint k1 k2 /\
+    live h k /\ live h r1 /\ live h r2 /\
+    disjoint k r1 /\ disjoint k r2 /\ disjoint r1 r2 /\
     qas_nat h k < S.q)
-  (ensures  fun h0 _ h1 -> modifies (loc k1 |+| loc k2) h0 h1 /\
-   (let k1_s, k2_s = SG.scalar_split_lambda (qas_nat h0 k) in
-    let k1 = qas_nat h1 k1 in let k2 = qas_nat h1 k2 in
-    k1 < S.q /\ k1 == k1_s /\ k2 < S.q /\ k2 == k2_s /\
-    k1 < pow2 129 /\ k2 < pow2 129))
+  (ensures  fun h0 _ h1 -> modifies (loc r1 |+| loc r2) h0 h1 /\
+   (let r1_s, r2_s = SG.scalar_split_lambda (qas_nat h0 k) in
+    let r1 = qas_nat h1 r1 in let r2 = qas_nat h1 r2 in
+    r1 < S.q /\ r1 == r1_s /\ r2 < S.q /\ r2 == r2_s /\
+    r1 < pow2 129 /\ r2 < pow2 129))
 
 [@CInline]
-let scalar_split_lambda k1 k2 k =
+let scalar_split_lambda r1 r2 k =
   let h0 = ST.get () in
   SGL.lemma_scalar_split_lambda_fits (qas_nat h0 k);
   push_frame ();
   let tmp1 = create_qelem () in
   let tmp2 = create_qelem () in
-  scalar_split_lambda_g1g2 tmp1 tmp2 k1 k2 k;
+  scalar_split_lambda_g1g2 tmp1 tmp2 r1 r2 k;
 
   make_minus_b1 tmp1; // tmp1 = minus_b1
   make_minus_b2 tmp2; // tmp2 = minus_b2
-  qmul k1 k1 tmp1; // k1 = c1 = c1 * minus_b1
-  qmul k2 k2 tmp2; // k2 = c2 = c2 * minus_b2
+  qmul r1 r1 tmp1; // r1 = c1 = c1 * minus_b1
+  qmul r2 r2 tmp2; // r2 = c2 = c2 * minus_b2
 
   make_minus_lambda tmp1; // tmp1 = minus_lambda
-  qadd k2 k1 k2; // k2 = r2 = c1 + c2
-  qmul tmp2 k2 tmp1; // tmp2 = r2 * minus_lambda
-  qadd k1 k tmp2; // k1 = r1 = k + r2 * minus_lambda
+  qadd r2 r1 r2; // r2 = r2 = c1 + c2
+  qmul tmp2 r2 tmp1; // tmp2 = r2 * minus_lambda
+  qadd r1 k tmp2; // r1 = r1 = k + r2 * minus_lambda
   pop_frame ()
 
+
+(**
+ Fast computation of [lambda]P as (beta * px, py, pz) in projective coordinates
+*)
 
 // [lambda]P = (beta * px, py, pz)
 val point_mul_lambda: res:point -> p:point -> Stack unit
@@ -129,7 +138,7 @@ let point_mul_lambda_inplace res =
 
 
 // // TODO: set it to a constant?
-// // [lambda]G
+// // [lambda]G = (beta * gx, gy, one)
 // inline_for_extraction noextract
 // val point_mul_g_lambda: res:point -> Stack unit
 //   (requires fun h -> live h res)
@@ -138,11 +147,34 @@ let point_mul_lambda_inplace res =
 //     point_eval h1 res == SG.point_mul_g_lambda ())
 
 // let point_mul_g_lambda res =
-//   push_frame ();
-//   let g = create_point () in
-//   PM.make_g g;
-//   point_mul_lambda res g;
-//   pop_frame ()
+//   PM.make_g res;
+//   point_mul_lambda_inplace res
+
+(**
+ Fast computation of [scalar]Q in projective coordinates
+*)
+
+inline_for_extraction noextract
+val point_mul_lambda_and_split_lambda:
+  r1:qelem -> r2:qelem -> lambda_q:point -> scalar:qelem -> q:point -> Stack unit
+  (requires fun h ->
+    live h r1 /\ live h r2 /\ live h lambda_q /\ live h scalar /\ live h q /\
+    disjoint r1 r2 /\ disjoint r1 lambda_q /\ disjoint r1 scalar /\ disjoint r1 q /\
+    disjoint r2 lambda_q /\ disjoint r2 scalar /\ disjoint r2 q /\
+    disjoint lambda_q scalar /\ disjoint lambda_q q /\
+    point_inv h q /\ qas_nat h scalar < S.q)
+  (ensures fun h0 _ h1 -> modifies (loc r1 |+| loc r2 |+| loc lambda_q) h0 h1 /\
+    point_inv h1 lambda_q /\
+    point_eval h1 lambda_q == SG.point_mul_lambda (point_eval h0 q) /\
+   (let r1_s, r2_s = SG.scalar_split_lambda (qas_nat h0 scalar) in
+    qas_nat h1 r1 < S.q /\ qas_nat h1 r1 < pow2 129 /\
+    qas_nat h1 r2 < S.q /\ qas_nat h1 r2 < pow2 129 /\
+    qas_nat h1 r1 == r1_s /\ qas_nat h1 r2 == r2_s))
+
+let point_mul_lambda_and_split_lambda r1 r2 lambda_q scalar q =
+  scalar_split_lambda r1 r2 scalar; // (r1 + r2 * lambda) % S.q = scalar
+  point_mul_lambda lambda_q q // lambda_q = [lambda]Q
+
 
 inline_for_extraction noextract
 let table1_inv_precomp (q:LSeq.lseq uint64 15) : BE.table_inv_t U64 15ul 16ul =
@@ -173,27 +205,47 @@ let lprecomp_get_consttime_lambda q ctx lambda_q table1 r_small res =
     SE.pow S.mk_k256_concrete_ops (point_eval_lseq lambda_q) (v r_small))
 
 
+// This function returns [r_small]([lambda]Q)
+// using a precomputed table [0; Q; 2Q; ...; 15Q]
 inline_for_extraction noextract
-val point_mul_split_lambda_table: out:point -> r1:qelem -> r2:qelem -> q:point -> Stack unit
+val lprecomp_get_vartime_lambda:
+  q:Ghost.erased (LSeq.lseq uint64 15){point_inv_lseq q} ->
+  BE.pow_a_to_small_b_st U64 15ul 0ul PM.mk_k256_concrete_ops 4ul 16ul (table1_inv_precomp q)
+
+let lprecomp_get_vartime_lambda q ctx lambda_q table1 r_small res =
+  let h0 = ST.get () in
+  assert (table1_inv_precomp q lambda_q (as_seq h0 table1));
+  // table1.[r_small] = [r_small]Q
+  BE.lprecomp_get_vartime 15ul 0ul PM.mk_k256_concrete_ops 4ul 16ul ctx q table1 r_small res;
+  let h1 = ST.get () in
+  assert (point_eval h1 res == SE.pow S.mk_k256_concrete_ops (point_eval_lseq q) (v r_small));
+  point_mul_lambda_inplace res;
+  let h2 = ST.get () in
+  assert (point_eval h2 res == SG.point_mul_lambda (point_eval h1 res));
+  // GLV lemma
+  assume (point_eval h2 res ==
+    SE.pow S.mk_k256_concrete_ops (point_eval_lseq lambda_q) (v r_small))
+
+
+inline_for_extraction noextract
+val point_mul_split_lambda_table:
+  out:point -> r1:qelem -> q1:point -> r2:qelem -> q2:point -> Stack unit
   (requires fun h ->
-    live h out /\ live h r1 /\ live h r2 /\ live h q /\
-    disjoint out q /\ disjoint out r1 /\ disjoint out r2 /\
-    disjoint q r1 /\ disjoint q r2 /\
-    point_inv h q /\
+    live h out /\ live h r1 /\ live h r2 /\ live h q1 /\ live h q2 /\
+    eq_or_disjoint q1 q2 /\ disjoint out q1 /\ disjoint out q2 /\
+    disjoint out r1 /\ disjoint out r2 /\
+    point_inv h q1 /\ point_inv h q2 /\
+    point_eval h q2 == SG.point_mul_lambda (point_eval h q1) /\
     qas_nat h r1 < S.q /\ qas_nat h r1 < pow2 129 /\
     qas_nat h r2 < S.q /\ qas_nat h r2 < pow2 129)
   (ensures  fun h0 _ h1 -> modifies (loc out) h0 h1 /\
     point_inv h1 out /\
     point_eval h1 out ==
-      SE.exp_double_fw S.mk_k256_concrete_ops (point_eval h0 q) 129
-        (qas_nat h0 r1) (SG.point_mul_lambda (point_eval h0 q)) (qas_nat h0 r2) 4)
+      SE.exp_double_fw S.mk_k256_concrete_ops
+        (point_eval h0 q1) 129 (qas_nat h0 r1)
+        (point_eval h0 q2) (qas_nat h0 r2) 4)
 
-let point_mul_split_lambda_table out r1 r2 q =
-  let h0 = ST.get () in
-  push_frame ();
-  let q2 = create_point () in
-  point_mul_lambda q2 q; // q2 = [lambda]Q
-
+let point_mul_split_lambda_table out r1 q1 r2 q2 =
   [@inline_let] let len = 15ul in
   [@inline_let] let ctx_len = 0ul in
   [@inline_let] let k = PM.mk_k256_concrete_ops in
@@ -201,27 +253,20 @@ let point_mul_split_lambda_table out r1 r2 q =
   [@inline_let] let table_len = 16ul in
   [@inline_let] let bLen = 4ul in
   [@inline_let] let bBits = 129ul in
-
+  let h0 = ST.get () in
+  push_frame ();
   let table1 = create (table_len *! len) (u64 0) in
-  PT.lprecomp_table len ctx_len k (null uint64) q table_len table1;
+  PT.lprecomp_table len ctx_len k (null uint64) q1 table_len table1;
 
   ME.mk_lexp_double_fw_tables len ctx_len k l table_len
     (BE.table_inv_precomp len ctx_len k l table_len)
-    (table1_inv_precomp (as_seq h0 q))
+    (table1_inv_precomp (as_seq h0 q1))
     (BE.lprecomp_get_consttime len ctx_len k l table_len)
-    (lprecomp_get_consttime_lambda (as_seq h0 q))
-    (null uint64) q bLen bBits r1 q2 r2 table1 table1 out;
-
-  //ME.lexp_double_fw_vartime 15ul 0ul PM.mk_k256_concrete_ops 4ul (null uint64)
-    //q 4ul 129ul r1 q2 r2 out;
-  let h1 = ST.get () in
-  assert (point_eval h1 out ==
-      SE.exp_double_fw S.mk_k256_concrete_ops (point_eval h0 q) 129
-        (qas_nat h0 r1) (SG.point_mul_lambda (point_eval h0 q)) (qas_nat h0 r2) 4);
+    (lprecomp_get_consttime_lambda (as_seq h0 q1))
+    (null uint64) q1 bLen bBits r1 q2 r2 table1 table1 out;
   pop_frame ()
 
 
-// TODO: share a table [0; P; 2P; ..; 15P] between P and ([lambda]P)
 // [scalar]Q = [(r1 + r2 * lambda) % S.q]Q = [r1]Q + [r2]([lambda]Q)
 val point_mul_split_lambda: out:point -> scalar:qelem -> q:point -> Stack unit
   (requires fun h ->
@@ -238,8 +283,9 @@ let point_mul_split_lambda out scalar q =
   push_frame ();
   let r1 = create_qelem () in
   let r2 = create_qelem () in
-  scalar_split_lambda r1 r2 scalar; // (r1 + r2 * lambda) % S.q = scalar
-  point_mul_split_lambda_table out r1 r2 q;
+  let q2 = create_point () in
+  point_mul_lambda_and_split_lambda r1 r2 q2 scalar q;
+  point_mul_split_lambda_table out r1 q r2 q2;
 
   assume (
     SGL.point_mul_split_lambda (qas_nat h0 scalar) (point_eval h0 q) ==
@@ -262,4 +308,135 @@ let point_mul_g_split_lambda out scalar =
   let g = create 15ul (u64 0) in
   PM.make_g g;
   point_mul_split_lambda out scalar g;
+  pop_frame ()
+
+
+(**
+ Fast computation of [scalar1]Q1 + [scalar2]Q2 in projective coordinates
+*)
+
+inline_for_extraction noextract
+val point_mul_double_split_lambda_table:
+    out:point
+  -> r1:qelem -> q1:point
+  -> r2:qelem -> q2:point
+  -> r3:qelem -> q3:point
+  -> r4:qelem -> q4:point ->
+  Stack unit
+  (requires fun h ->
+    live h out /\ live h r1 /\ live h r2 /\ live h r3 /\ live h r4 /\
+    live h q1 /\ live h q2 /\ live h q3 /\ live h q4 /\
+    eq_or_disjoint q1 q2 /\ eq_or_disjoint q1 q3 /\ eq_or_disjoint q1 q4 /\
+    eq_or_disjoint q2 q3 /\ eq_or_disjoint q2 q4 /\ eq_or_disjoint q3 q4 /\
+    disjoint out q1 /\ disjoint out q2 /\ disjoint out q3 /\ disjoint out q4 /\
+    disjoint out r1 /\ disjoint out r2 /\ disjoint out r3 /\ disjoint out r4 /\
+    point_inv h q1 /\ point_inv h q2 /\ point_inv h q3 /\ point_inv h q4 /\
+    point_eval h q2 == SG.point_mul_lambda (point_eval h q1) /\
+    point_eval h q4 == SG.point_mul_lambda (point_eval h q3) /\
+    qas_nat h r1 < S.q /\ qas_nat h r1 < pow2 129 /\
+    qas_nat h r2 < S.q /\ qas_nat h r2 < pow2 129 /\
+    qas_nat h r3 < S.q /\ qas_nat h r3 < pow2 129 /\
+    qas_nat h r4 < S.q /\ qas_nat h r4 < pow2 129)
+  (ensures  fun h0 _ h1 -> modifies (loc out) h0 h1 /\
+    point_inv h1 out /\
+    point_eval h1 out ==
+      SE.exp_four_fw S.mk_k256_concrete_ops
+        (point_eval h0 q1) 129 (qas_nat h0 r1)
+        (point_eval h0 q2) (qas_nat h0 r2)
+        (point_eval h0 q3) (qas_nat h0 r3)
+        (point_eval h0 q4) (qas_nat h0 r4) 4)
+
+let point_mul_double_split_lambda_table out r1 q1 r2 q2 r3 q3 r4 q4 =
+  [@inline_let] let len = 15ul in
+  [@inline_let] let ctx_len = 0ul in
+  [@inline_let] let k = PM.mk_k256_concrete_ops in
+  [@inline_let] let l = 4ul in
+  [@inline_let] let table_len = 16ul in
+  [@inline_let] let bLen = 4ul in
+  [@inline_let] let bBits = 129ul in
+  let h0 = ST.get () in
+  push_frame ();
+  let table1 = create (table_len *! len) (u64 0) in
+  PT.lprecomp_table len ctx_len k (null uint64) q1 table_len table1;
+  let h1 = ST.get () in
+  assert (BE.table_inv_precomp len ctx_len k l table_len
+    (as_seq h1 q1) (as_seq h1 table1));
+
+  let table3 = create (table_len *! len) (u64 0) in
+  PT.lprecomp_table len ctx_len k (null uint64) q3 table_len table3;
+  let h2 = ST.get () in
+  assert (BE.table_inv_precomp len ctx_len k l table_len
+    (as_seq h2 q1) (as_seq h2 table1));
+  assert (table1_inv_precomp (as_seq h2 q1)
+    (as_seq h2 q2) (as_seq h2 table1));
+  assert (BE.table_inv_precomp len ctx_len k l table_len
+    (as_seq h2 q3) (as_seq h2 table3));
+  assert (table1_inv_precomp (as_seq h2 q3)
+    (as_seq h2 q4) (as_seq h2 table3));
+
+  ME.mk_lexp_four_fw_tables len ctx_len k l table_len
+    (BE.table_inv_precomp len ctx_len k l table_len)
+    (table1_inv_precomp (as_seq h2 q1))
+    (BE.table_inv_precomp len ctx_len k l table_len)
+    (table1_inv_precomp (as_seq h2 q3))
+    (BE.lprecomp_get_vartime len ctx_len k l table_len)
+    (lprecomp_get_vartime_lambda (as_seq h2 q1))
+    (BE.lprecomp_get_vartime len ctx_len k l table_len)
+    (lprecomp_get_vartime_lambda (as_seq h2 q3))
+    (null uint64) q1 bLen bBits r1 q2 r2 q3 r3 q4 r4
+    table1 table1 table3 table3 out;
+
+  pop_frame ()
+
+
+val point_mul_double_split_lambda_vartime:
+  out:point -> scalar1:qelem -> q1:point -> scalar2:qelem -> q2:point -> Stack unit
+  (requires fun h ->
+    live h out /\ live h scalar1 /\ live h q1 /\ live h scalar2 /\ live h q2 /\
+    disjoint q1 out /\ disjoint q2 out /\ eq_or_disjoint q1 q2 /\
+    disjoint scalar1 out /\ disjoint scalar2 out /\
+    point_inv h q1 /\ point_inv h q2 /\
+    qas_nat h scalar1 < S.q /\ qas_nat h scalar2 < S.q)
+  (ensures fun h0 _ h1 -> modifies (loc out) h0 h1 /\
+    point_inv h1 out /\
+    point_eval h1 out ==
+    S.point_mul_double
+      (qas_nat h0 scalar1) (point_eval h0 q1)
+      (qas_nat h0 scalar2) (point_eval h0 q2))
+
+[@CInline]
+let point_mul_double_split_lambda_vartime out scalar1 q1 scalar2 q3 =
+  let h0 = ST.get () in
+  push_frame ();
+  let r1 = create_qelem () in
+  let r2 = create_qelem () in
+  let r3 = create_qelem () in
+  let r4 = create_qelem () in
+  let q2 = create_point () in
+  let q4 = create_point () in
+  point_mul_lambda_and_split_lambda r1 r2 q2 scalar1 q1;
+  point_mul_lambda_and_split_lambda r3 r4 q4 scalar2 q3;
+  point_mul_double_split_lambda_table out r1 q1 r2 q2 r3 q3 r4 q4; admit();
+  pop_frame ()
+
+
+val point_mul_g_double_split_lambda_vartime:
+  out:point -> scalar1:qelem -> scalar2:qelem -> q2:point ->
+  Stack unit
+  (requires fun h ->
+    live h out /\ live h scalar1 /\ live h scalar2 /\ live h q2 /\
+    disjoint q2 out /\ disjoint out scalar1 /\ disjoint out scalar2 /\
+    point_inv h q2 /\ qas_nat h scalar1 < S.q /\ qas_nat h scalar2 < S.q)
+  (ensures fun h0 _ h1 -> modifies (loc out) h0 h1 /\
+    point_inv h1 out /\
+    point_eval h1 out ==
+    S.point_mul_double_g
+      (qas_nat h0 scalar1) (qas_nat h0 scalar2) (point_eval h0 q2))
+
+[@CInline]
+let point_mul_g_double_split_lambda_vartime out scalar1 scalar2 q2 =
+  push_frame ();
+  let g = create 15ul (u64 0) in
+  PM.make_g g;
+  point_mul_double_split_lambda_vartime out scalar1 g scalar2 q2;
   pop_frame ()
