code/k256/Hacl.Impl.K256.Verify.fst
@@ -15,6 +15,7 @@ module KL = Spec.K256.Lemmas
 open Hacl.K256.Field
 open Hacl.Impl.K256.Point
 open Hacl.Impl.K256.PointMul
+open Hacl.Impl.K256.GLV
 
 module QA = Hacl.K256.Scalar
 module QI = Hacl.Impl.K256.Qinv
@@ -67,7 +68,8 @@ let ecdsa_verify_qelem res p z r s =
   QI.qinv sinv s;
   QA.qmul u1 z sinv;
   QA.qmul u2 r sinv;
-  point_mul_g_double_vartime res u1 u2 p;
+  //point_mul_g_double_vartime res u1 u2 p;
+  point_mul_g_double_split_lambda_vartime res u1 u2 p;
   pop_frame ()
 
 
